

Homework 2
Asiaiah Crutchfield – 1133547

$$ddx [(4x^3+x)(2x^4-x^2+2)]$$

Product rule:

$$\begin{aligned} 4x^3+x &= 12x^2 + 1 \mid 2x^4 - x^2 + 2 = 8x^3 - 2x \\ (12x^2 + 1)(2x^4 - x^2 + 2) &+ (8x^3 - 2x)(4x^3+x) \\ (24x^6 - 10x^4 + 23x^2 + 2) &+ (32x^6 - 2x) \\ 56x^6 - 10x^4 + 21x^2 + 2 \end{aligned}$$

$$ddx(4k/7x^8), k \text{ is a constant}$$

Constant multiplication rule:

$$\begin{aligned} 4k/7x^8 &= (4k/7)(-8x^{-9}) \\ -32k/7x^9 &= -32k/7x^9 \end{aligned}$$

$$ddx(3x^2+1/x+4)$$

Quotient rule:

$$\begin{aligned} 3x^2+1/x+4 &= 6x/1 \\ x+4(6x)-(3x^2+1)(1)/(x+4)^2 &= 6x^2+24x-(3x^2+1)/(x+4)^2 \\ 3x^2+24x-1/(x+4)^2 \end{aligned}$$

$$ddx(x^2+3\sqrt{2x+(x^2+1)})^{10}$$

$$(x^2+3\sqrt{2x+(x^2+1)})^{10} = 3(2x+(x^2+1))^{1/2}$$

Chain rule:

$$\begin{aligned} 3 \cdot 1/2(2x+(x^2+1))^{-1/2} \cdot 2+2x &= 3/2\sqrt{2x+(x^2+1)} \cdot (2+2x) \\ 10 \cdot (x^2+3\sqrt{2x+(x^2+1)})^9 \cdot (2x+2\sqrt{2x+(x^2+1)} \cdot (2+2x)) \end{aligned}$$

$$ddx \sin(\cos(\tan(x)))$$

Chain rule:

$$(\cos(\tan(x))) = -\cos(\cos(\tan(x))) \cdot \sin(\tan(x)) \cdot \sec^2(x)$$

$$4x^2y - 2y = x^3 + 2, \quad dy/dx = ?$$

Product rule:

$$4x^2y - 2y = x^3 + 2 \rightarrow 8xy + 4x^2(dy/dx) - 2(dy/dx) = 3x^2$$

$$4x^2(dy/dx) - 2(dy/dx) = 3x^2 - 8xy \rightarrow (dy/dx)(4x^2 - 2) = 3x^2 - 8xy$$

$$dy/dx = (3x^2 - 8xy) / (4x^2 - 2)$$

$$x^2y + y^3 = \sin(x), \quad dy/dx = ?$$

Product rule:

$$2xy + x^2(dy/dx) + 3y^2(dx/dy) + 3y^2(dx/dy) = \cos(x)$$

$$x^2(dx/dy) + 3y^2(dx/dy) = \cos(x) - 2xy$$

$$(dx/dy)(x^2 + 3y^2) = \cos(x) - 2xy$$

$$dx/dy = (\cos(x) - 2xy) / (x^2 + 3y^2)$$

$$\sin(\cos(x+y)) = x^2 + y^2, \quad dy/dx = ?$$

$$\cos(\cos(x+y))(-\sin(x+y) \cdot (1 + dx/dy)) = 2x + 2y(dx/dy)$$

$$-\cos(\cos(x+y)) \cdot \sin(x+y) - \cos(\cos(x+y)) \cdot \sin(x+y) \cdot dx/dy = 2x + 2y(dx/dy)$$

$$-\cos(\cos(x+y)) \cdot \sin(x+y) \cdot dx/dy - 2y(dx/dy) = 2x + \cos(\cos(x+y)) \cdot \sin(x+y)$$

$$dx/dy \cdot (-\cos(\cos(x+y)) \cdot \sin(x+y) - 2y) = 2x + \cos(\cos(x+y)) \cdot \sin(x+y)$$

$$dx/dy = (-\cos(\cos(x+y)) \cdot \sin(x+y) - 2y) / (2x + \cos(\cos(x+y)) \cdot \sin(x+y))$$

$$\tan^2(xy) + \csc^2(x+y) = 1, \quad dy/dx = ?$$

Product rule:

$$d/dx(\tan^2(xy)) = 2\tan(xy) \cdot \sec^2(xy) \cdot (x(dx/dy) + y)$$

$$dx/dx(\csc^2(x+y)) = -2\csc^2(x+y) \cdot \cot(x+y) \cdot (1 + dx/dy)$$

$$2\tan(xy) \cdot \sec^2(xy) \cdot (x(dx/dy) + y) - 2\csc^2(x+y) \cdot \cot(x+y) \cdot (1 + dx/dy) = 0$$

$$2\tan(xy) \cdot \sec^2(xy) \cdot x(dy/dx) - 2\csc^2(x+y) \cdot \cot(x+y) \cdot dy/dx =$$

$$-2\tan(xy) \cdot \sec^2(xy) \cdot y + 2\csc^2(x+y) \cdot \cot(x+y)$$

$$dy/dx(2\tan(xy) \cdot \sec^2(xy) \cdot x - 2\csc^2(x+y) \cdot \cot(x+y)) =$$

$$-2\tan(xy) \cdot \sec^2(xy) \cdot y + 2\csc^2(x+y) \cdot \cot(x+y)$$

$$dy/dx = (-2\tan(xy) \cdot \sec^2(xy) \cdot y + 2\csc^2(x+y) \cdot \cot(x+y)) /$$

$$2\tan(xy) \cdot \sec^2(xy) \cdot x - 2\csc^2(x+y) \cdot \cot(x+y)$$